minor naming changes

DiagonaLean/UTMHalt/Basic.lean
@@ -29,7 +29,7 @@ def IsHaltDeciderFor (U D : SingleTapeTM Bool) : Prop :=
   ∀ x : List Bool, (Halts U x → D.Outputs x [true]) ∧ (¬ Halts U x → D.Outputs x [false])
 
 /-- The `Halts` predicate for Weak UTMs. -/
-def UTMWeaklyHalts (U : SingleTapeTM Bool) (_hU : IsWeaklyUniversal U) (M : SingleTapeTM Bool)
+def WeakUTMHalts (U : SingleTapeTM Bool) (_hU : IsWeaklyUniversal U) (M : SingleTapeTM Bool)
   (w : List Bool) [DecidableEq M.State] := Halts U (instanceEncoding M w)
 
 /-- The `Halts` predicate for UTMs. -/
@@ -37,12 +37,12 @@ def UTMHalts (U : SingleTapeTM Bool) (_hU : IsUniversal U) (M : SingleTapeTM Boo
   (w : List Bool) [DecidableEq M.State] := Halts U (instanceEncoding M w)
 
 /-- The halting problem of the fixed Weak UTM `U`. -/
-abbrev WeakUniversalHaltProblem : ({U : SingleTapeTM Bool // IsWeaklyUniversal U} ×
+abbrev WeakUTMHaltProblem : ({U : SingleTapeTM Bool // IsWeaklyUniversal U} ×
     Σ (M : SingleTapeTM Bool), DecidableEq M.State × List Bool) → Prop := 
-  fun ⟨⟨U, hU⟩, ⟨M, _inst, w⟩⟩ ↦ UTMWeaklyHalts U hU M w
+  fun ⟨⟨U, hU⟩, ⟨M, _inst, w⟩⟩ ↦ WeakUTMHalts U hU M w
 
 /-- The halting problem of the fixed UTM `U`. -/
-abbrev UniversalHaltProblem : ({U : SingleTapeTM Bool // IsUniversal U} ×
+abbrev UTMHaltProblem : ({U : SingleTapeTM Bool // IsUniversal U} ×
     Σ (M : SingleTapeTM Bool), DecidableEq M.State × List Bool) → Prop := 
   fun ⟨⟨U, hU⟩, ⟨M, _inst, w⟩⟩ ↦ UTMHalts U hU M w
 
